README.md
@@ -20,7 +20,7 @@ Compatible with Coq 8.20.0 and MetaCoq 1.3.2.
 - [x] Add pragma for program selection
 - [x] Make pretty-printer prettier
 - [x] Ensure well-formedness of generated programs inside Coq
-  - [ ] Make well-formedness check faster by splitting it into boolean and propositional.
+  - [x] Make well-formedness check faster by splitting it into boolean and propositional.
 - [ ] Evaluate λ□ programs from inside Coq to start testing
   - [ ] Possibly salvage an existing interpreter
   - [ ] Or implement our own...
